Progress towards GVN.

GVN.v
@@ -1,7 +1,7 @@
 Require Import CSet Le.
 
 Require Import Plus Util AllInRel Map.
-Require Import Val Var Env EnvTy IL ParamsMatch Sim SimApx Alpha Coherence Fresh Annotation.
+Require Import Val Var Env EnvTy IL ParamsMatch Sim SimApx Alpha Coherence Fresh Annotation MoreExp.
 
 Require Import Liveness Filter.
 
@@ -11,7 +11,8 @@ Unset Printing Records.
 
 Definition eqn := (exp * exp)%type.
 
-Instance OrderedType eqn : OrderedType eqn.
+Instance OrderedType : OrderedType exp.
+
 Admitted.
 
 Definition satisfies (E:onv val) (gamma:eqn) := 
@@ -24,20 +25,26 @@ Inductive moreDef {X} : option X -> option X -> Prop :=
 Definition satisfiesAll (E:onv val) (Gamma:set eqn) := 
   forall gamma, gamma ∈ Gamma -> satisfies E gamma.
 
-Definition entails Gamma Γ' := forall E, satisfiesAll E Gamma -> satisfiesAll E Γ'. 
+Definition sem_entails Gamma Γ' := forall E, satisfiesAll E Gamma -> satisfiesAll E Γ'. 
 
-Definition moreDefined Gamma e e' := 
-  forall E E', satisfiesAll E Gamma -> satisfiesAll E' Gamma -> fstNoneOrR eq (exp_eval E e) (exp_eval E' e').
+Definition freeVars (gamma:exp * exp) := 
+  Exp.freeVars (fst gamma) ∪ Exp.freeVars (snd gamma).
 
-Definition moreDefinedArgs Gamma Y Y' := 
-  forall E E', satisfiesAll E Gamma -> satisfiesAll E' Gamma -> 
+Definition eqns_freeVars (Gamma:set eqn) := fold union (map freeVars Gamma) ∅.
+
+Definition entails Gamma Γ' := (forall E, satisfiesAll E Gamma -> satisfiesAll E Γ') 
+/\ eqns_freeVars Γ' ⊆ eqns_freeVars Gamma. 
+
+Definition moreDefined Gamma Γ' e e' := 
+  forall E E', satisfiesAll E Gamma -> satisfiesAll E' Γ' -> fstNoneOrR eq (exp_eval E e) (exp_eval E' e').
+
+Definition moreDefinedArgs Gamma Γ' Y Y' := 
+  forall E E', satisfiesAll E Gamma -> satisfiesAll E' Γ' -> 
           fstNoneOrR eq (omap (exp_eval E) Y) (omap (exp_eval E') Y').
 
 (*Definition moreDefined Gamma Γ' e e' := 
   forall E, satisfies E Gamma -> forall E', satisfies E' Γ' -> moreDef (exp_eval E e) (exp_eval E' e').*)
 
-Definition freeVars (gamma:exp * exp) := 
-  Exp.freeVars (fst gamma) ∪ Exp.freeVars (snd gamma).
 
 Definition remove (Gamma:set eqn) G :=
   filter (fun gamma => B[freeVars gamma ∩ G [=] ∅]) Gamma.
@@ -50,44 +57,50 @@ Definition subst_eqns (ϱ : env exp) (G:set eqn) :=
 
 Definition sid := fun x => Var x.
 
-Definition eqns_freeVars (Gamma:set eqn) := fold union (map freeVars Gamma) ∅.
 
-Inductive eqn_sound : list (params*set eqn) 
+Inductive eqn_sound : list (params*set eqn*set eqn*set eqn*set eqn) 
                       -> stmt 
+                      -> ann (set eqn) 
                       -> ann (set eqn) 
                       -> ann (list exp) 
                       -> Prop :=
-| EqnOpr x Lv b e al Gamma e' al' 
-  : eqn_sound Lv b al al'
+| EqnOpr x Lv b e Gamma al Γ' (al':ann (set eqn)) e' al' cl
+  : eqn_sound Lv b al al' cl
     (* make sure the rest conforms to the new assignment *)
     -> entails (Gamma ∪ {{ (Var x,e) }}) (getAnn al)
-    -> moreDefined Gamma e e'
-    -> eqns_freeVars (getAnn al) [<=] eqns_freeVars Gamma ++ {x; {}}
-    -> eqn_sound Lv (stmtExp x e b) (ann1 Gamma al) (ann1 (e'::nil) al')
-| EqnIf Lv e e' b1 b2 Gamma al1 al2 al1' al2'
-  : eqn_sound Lv b1 al1 al1'
-  -> eqn_sound Lv b2 al2 al2'
+    -> entails (Γ' ∪ {{ (Var x,e') }}) (getAnn al')
+    -> moreDefined Gamma Γ' e e'
+    -> eqn_sound Lv (stmtExp x e b) (ann1 Gamma al) (ann1 Γ' al') (ann1 (e'::nil) cl)
+| EqnIf Lv e e' b1 b2 Gamma Γ' al1 al2 al1' al2' cl1 cl2
+  : eqn_sound Lv b1 al1 al1' cl1
+  -> eqn_sound Lv b2 al2 al2' cl2
+ (* TODO: include information about condition *)
   -> entails Gamma (getAnn al1)
   -> entails Gamma (getAnn al2)
-  -> eqns_freeVars (getAnn al1)[<=]eqns_freeVars Gamma
-  -> eqns_freeVars (getAnn al2)[<=]eqns_freeVars Gamma
-  -> moreDefined Gamma e e'
-  -> eqn_sound Lv (stmtIf e b1 b2) (ann2 Gamma al1 al2) (ann2 (e'::nil) al1' al2')
-| EqnGoto l Y Y' Lv Gamma Z EqS
-  : get Lv (counted l) (Z,EqS)
+  -> entails Γ' (getAnn al1')
+  -> entails Γ' (getAnn al2')
+  -> moreDefined Gamma Γ' e e'
+  -> eqn_sound Lv (stmtIf e b1 b2) (ann2 Gamma al1 al2) (ann2 Γ' al1' al2') (ann2 (e'::nil) cl1 cl2)
+| EqnGoto l Y Y' Lv Gamma Γ' Z Γf Γf' EqS EqS'
+  : get Lv (counted l) (Z,Γf, EqS, Γf',EqS')
     -> length Y = length Y'
-    -> entails Gamma (subst_eqns (sid [Z <-- Y']) EqS)
-    -> moreDefinedArgs Gamma Y Y'
-    -> eqn_sound Lv (stmtGoto l Y) (ann0 Gamma) (ann0 Y')
-| EqnReturn Lv e e' Gamma
-  : entails Gamma {{(e,e')}}
-    -> eqn_sound Lv (stmtReturn e') (ann0 Gamma) (ann0 (e::nil))
-| EqnLet Lv s Z b Gamma EqS als alb als' alb'
-  : eqn_sound ((Z,EqS)::Lv) s als als'
-  -> eqn_sound ((Z,EqS)::Lv) b alb alb'
-  -> entails (Gamma ∪ EqS) (getAnn alb)
+    -> entails Gamma (subst_eqns (sid [Z <-- Y]) EqS)
+    -> entails Γ' (subst_eqns (sid [Z <-- Y']) EqS')
+    -> moreDefinedArgs Gamma Γ' Y Y'
+    -> eqn_sound Lv (stmtGoto l Y) (ann0 Gamma) (ann0 Γ') (ann0 Y')
+| EqnReturn Lv e e' Gamma Γ'
+  : moreDefined Gamma Γ' e e'
+    -> eqn_sound Lv (stmtReturn e) (ann0 Gamma) (ann0 Γ') (ann0 (e'::nil))
+| EqnLet Lv s Z b Gamma Γ' EqS EqS' als alb als' alb' cls clb
+  : eqn_sound ((Z,Gamma, EqS, Γ', EqS')::Lv) s als als' cls
+  -> eqn_sound ((Z,Gamma, EqS, Γ', EqS')::Lv) b alb alb' clb
+  -> entails (Gamma ∪ EqS) (getAnn als)
   -> entails Gamma (getAnn alb)
-  -> eqn_sound Lv (stmtLet Z s b) (ann2 Gamma als alb) (ann2 nil als' alb').
+  -> entails (Γ' ∪ EqS') (getAnn als')
+  -> entails Γ' (getAnn alb')
+  -> eqns_freeVars EqS ⊆ eqns_freeVars Gamma ++ of_list Z
+  -> eqns_freeVars EqS' ⊆ eqns_freeVars Γ' ++ of_list Z
+  -> eqn_sound Lv (stmtLet Z s b) (ann2 Gamma als alb) (ann2 Γ' als' alb') (ann2 nil cls clb).
 
 Fixpoint compile (s:stmt) (a:ann (list exp)) :=
   match s, a with
@@ -103,15 +116,19 @@ Fixpoint compile (s:stmt) (a:ann (list exp)) :=
     | s, _ => s
   end.
 
-Definition ArgRel (G:(params * set eqn)) (VL VL': list val) : Prop := 
-  True.
+Definition ArgRel (G:list var*set eqn*set eqn*set eqn*set eqn) (VL VL': list val) : Prop := 
+  let '(Z, Gamma, EqS, Γ', EqS') := G in
+  length Z = length VL 
+  /\ length VL = length VL' 
+  /\ (forall E:onv val, satisfiesAll E Gamma -> 
+                  satisfiesAll (E[Z <-- List.map Some VL]) (Gamma ∪ EqS))
+  /\ (forall E:onv val, satisfiesAll E Γ' -> 
+                  satisfiesAll (E[Z <-- List.map Some VL']) (Γ' ∪ EqS')).
 
-Definition ParamRel (G:(params * set eqn)) (Z Z' : list var) : Prop := 
-  Z = Z'.
 
-
-Definition blockRel (AL:list (params*set eqn)) (L:F.labenv) (L':F.labenv) := 
-  forall n blk lvZ, get AL n lvZ -> get L n blk -> True.
+Definition ParamRel (G:params*set eqn*set eqn*set eqn*set eqn) (Z Z' : list var) : Prop := 
+  let '(Zb, Gamma, EqS, Γ', EqS') := G in  
+  Z = Z' /\ Zb = Z.
 
 
 (* problem is Gamma that satisfies nothing 
@@ -132,69 +149,179 @@ Proof.
 Qed.
 *)
 
-Lemma sim_DVE r L L' V V' s LV eqns repl G G'
+Lemma eqns_freeVars_add Gamma x e
+  : eqns_freeVars (Gamma ++ {{(Var x, e)}}) [=] eqns_freeVars (Gamma) ∪ {{ x }} ∪ Exp.freeVars e.
+Proof.
+Admitted.
+
+Lemma eqns_freeVars_union Gamma Γ'
+  : eqns_freeVars (Gamma ++ Γ') [=] eqns_freeVars (Gamma) ∪ eqns_freeVars Γ'.
+Proof.
+Admitted.
+
+Ltac dowith c t :=
+  match goal with 
+    | [ H : c _ _ _ _ |- _ ] => t H
+  end.
+
+Lemma sim_DVE r L L' V V' s LV eqns eqns' repl G G'
 :
   satisfiesAll V (getAnn eqns) 
--> satisfiesAll V' (getAnn eqns)
--> eqn_sound LV s eqns repl
+-> satisfiesAll V' (getAnn eqns')
+-> eqn_sound LV s eqns eqns' repl
 -> simL' r ArgRel ParamRel LV L L'
 -> ssa G s G'
 -> eqns_freeVars (getAnn eqns) ⊆ G
 -> paco2 (@psimapx F.state _ F.state _) r (L,V, s) (L',V', compile s repl).
 Proof.
   general induction s; simpl; invt eqn_sound; invt ssa; simpl in * |- *.
-  + specialize (H13 V V'). exploit H13; eauto. inv X.
+  + unfold moreDefined in H15; exploit H15; eauto. inv X.
     - pfold. econstructor 3; try eapply star_refl; eauto. stuck.
     - pfold. econstructor; try eapply plusO.
       econstructor; eauto using eq_sym.
       econstructor; eauto using eq_sym.
       left. eapply IHs; eauto.
-      eapply H10. admit. eapply H10. admit. 
-      rewrite <- H4. eauto.
-  + specialize (H17 V V'). exploit H17; eauto. inv X.
+      eapply H10. admit. eapply H14. admit.
+      destruct H10. rewrite eqns_freeVars_add in H9.
+      rewrite H9. rewrite H13. rewrite H4. clear_all; cset_tac; intuition.
+  + unfold moreDefined in H18; exploit H18; eauto. inv X.
     - pfold. econstructor 3; try eapply star_refl; eauto. stuck.
     - pfold. case_eq (val2bool y); intros. 
       econstructor; try eapply plusO.
       econstructor; eauto using eq_sym.
       econstructor; eauto using eq_sym.
-      left. eapply IHs1; eauto.
-      rewrite <- H4; eauto. 
+      left. eapply IHs1; eauto. 
+      eapply H10; eauto.
+      eapply H13; eauto.
+      destruct H10. rewrite <- H4; eauto. 
       econstructor; try eapply plusO.
       econstructor 3; eauto using eq_sym.
       econstructor 3; eauto using eq_sym.
       left. eapply IHs2; try eapply H9; eauto.
-      rewrite <- H4; eauto. 
+      eapply H11; eauto.
+      eapply H17; eauto.
+      destruct H11. rewrite <- H4; eauto.
   + destruct (get_dec L (counted l)) as [[[bE bZ bs]]|].
     (* hnf in H2. exploit H2; eauto. simpl in *. subst bZ. *)
-    (*    decide (length Z = length Y). *)
-    specialize (H13 V V'). exploit H13; eauto. inv X.
+    decide (length bZ = length Y).
+    hnf in H15. exploit H15; eauto. inv X.
     - pfold. econstructor 3; try eapply star_refl. eauto. stuck.
-    - unfold simL in H1.
-      edestruct AIR5_length; try eassumption; dcr.
+    - edestruct AIR5_length; try eassumption; dcr.
       edestruct get_length_eq; try eassumption.
       edestruct AIR5_nth as [?[? [?]]]; try eassumption; dcr. 
       simpl in *. repeat get_functional; subst.
-      inv H23. hnf in H27. subst bZ.
-      eapply sim_drop_shift. eapply H28; eauto. eapply I.
+      inv H24. hnf in H28; simpl in H28; dcr; subst.
+      eapply sim_drop_shift. eapply H29; eauto. hnf. simpl; repeat split. 
+      exploit omap_length; eauto. unfold var in *. rewrite e. congruence.
+      intros. hnf in H9. dcr.
+      Lemma satisfiesAll_subst E Z EqS Y Γf y
+      :  length Z = length Y
+         -> eqns_freeVars EqS ⊆ eqns_freeVars Γf ∪ of_list Z
+         -> eqns_freeVars Γf ∩ of_list Z = ∅
+         -> ⎣y ⎦ = omap (exp_eval E) Y
+         -> satisfiesAll E Γf
+         -> satisfiesAll E (subst_eqns (sid [Z <-- Y]) EqS)
+         -> satisfiesAll (E [Z <-- List.map Some y]) (Γf ++ EqS).
+      Proof.
+        intros.
+        Lemma satisfiesAll_union E Gamma Γ'
+              : satisfiesAll E (Gamma ∪ Γ')
+                <-> satisfiesAll E Gamma /\ satisfiesAll E Γ'.
+        Proof.
+          split.
+          intros H; split; hnf; intros; eapply H; cset_tac; intuition.
+          intros [A B]; hnf; intros. cset_tac. destruct H; auto.
+        Qed.
+        eapply satisfiesAll_union; split.
+        Lemma satisfiesAll_update_dead E Gamma Z vl
+        : length Z = length vl
+          -> satisfiesAll E Gamma
+          -> eqns_freeVars Gamma ∩ of_list Z = ∅
+          -> satisfiesAll (E[Z <-- vl]) Gamma.
+        Proof.
+          intros. hnf; intros. hnf; intros.
+          hnf in H; exploit H; eauto. hnf in X.
+          erewrite exp_eval_agree; try eapply X.
+          symmetry. 
+          erewrite exp_eval_agree; try eapply X; eauto using eq_sym.
+          symmetry. 
+          erewrite <- minus_inane_set.
+          eapply update_with_list_agree_minus; eauto. reflexivity.
+          exfalso; admit.
+          erewrite <- minus_inane_set.
+          symmetry.
+          eapply update_with_list_agree_minus; eauto. reflexivity.
+          exfalso; admit.
+          eapply H0; eauto.
+        Qed.
+        eapply satisfiesAll_update_dead; eauto. 
+        rewrite map_length; eauto.
+        exploit omap_length; eauto. congruence.
+        revert_except EqS. pattern EqS.
+        eapply set_induction; intros. 
+        - hnf; intros. exfalso.  eapply H. eapply H6.
+        - hnf; intros. rewrite Add_Equal in H1.
+          rewrite H1 in H8. eapply add_iff in H8. destruct H8.
+          hnf. hnf in H7.
+          unfold satisfies in H7.
+          specialize (H7 (subst_eqn (sid [Z <-- Y]) x)).
+          Lemma eval_exp_subst E y Y Z e
+          : length Z = length Y
+            -> ⎣y ⎦ = omap (exp_eval E) Y
+            -> exp_eval (E [Z <-- List.map Some y]) e = 
+              exp_eval E (subst_exp (sid [Z <-- Y]) e). 
+          Proof.
+            general induction e; simpl; eauto.
+            decide (v ∈ of_list Z).
+            eapply length_length_eq in H.
+            general induction H; simpl in * |- *; eauto.
+            symmetry in H0. monad_inv H0. simpl.
+            lud; eauto. eapply IHlength_eq; eauto.
+            cset_tac; intuition.
+            remember (sid [Z <-- Y] v); intros. symmetry in Heqy0; eauto.
+            eapply update_with_list_lookup_not_in in Heqy0. 
+            remember (E [Z <-- List.map Some y] v); intros. 
+            symmetry in Heqy1.
+            eapply update_with_list_lookup_not_in in Heqy1; eauto.
+            subst; simpl; eauto. eauto.
+            erewrite IHe1; eauto.
+            erewrite IHe2; eauto.
+          Qed.
+          intros. assert (x = gamma) by admit. subst gamma.
+          repeat erewrite eval_exp_subst; eauto. eapply H7.
+          eapply map_1. admit. rewrite H1. cset_tac; eauto.
+          eapply H; eauto. rewrite <- H3. admit.
+          hnf; intros. eapply H7. admit.
+      Qed.
+      eapply satisfiesAll_subst; eauto.
+      admit. admit.
+
     - pfold. econstructor 3; try eapply star_refl. eauto. stuck; eauto.
-  + pfold. econstructor 2; try eapply star_refl.
-    simpl. eapply H7 in H.
-    eapply H7. rewrite H; eauto. simpl. 
-    stuck. stuck.
+      get_functional; subst. simpl in *. congruence.
+    - pfold. econstructor 3; try eapply star_refl. eauto. stuck; eauto.
+  + simpl. hnf in H7; exploit H7; eauto. inv X; eauto.
+    - pfold. econstructor 3; try eapply star_refl. simpl. congruence.
+      stuck.
+    - pfold. econstructor 2; try eapply star_refl. simpl. congruence.
+      stuck. stuck.
   + pfold. econstructor; try eapply plusO.
     econstructor; eauto.
     econstructor; eauto.
-    simpl. left. eapply IHs2; eauto. 
-    - simpl in *; eapply agree_on_incl; eauto.
+    simpl. left. eapply IHs2; eauto.
+    - eapply H11; eauto.
+    - eapply H14; eauto.
     - eapply simL_mon; eauto. eapply simL_extension'; eauto.
-      hnf; intros. hnf in H3. hnf in H2. dcr; subst.
-      split; eauto. eapply filter_filter_by_length; eauto.
-      hnf; intros.
-      eapply IHs1; eauto.
-      * hnf in H2. dcr; subst. simpl.
-        eapply agree_on_update_filter'. eauto.
-        eapply agree_on_incl; eauto.
-      * split; reflexivity.
+      * hnf; intros. destruct a as [[[[Zb Γb] EqSb] Γb'] EqSb'].
+        hnf in H5. hnf in H6. dcr; subst.
+        split; eauto. unfold var in *. congruence.
+      * hnf; intros. hnf in H5; dcr.
+        eapply IHs1; eauto.
+        eapply H10. specialize (H23 V). eapply H23; eauto.
+        eapply H12. eapply H26; eauto.
+        destruct H10. rewrite H10. rewrite eqns_freeVars_union.
+         rewrite H18. rewrite H4. clear_all; cset_tac; intuition.
+      * hnf; split; eauto.
+    - destruct H11. rewrite H6; eauto.
 Qed.
 
 Print Assumptions sim_DVE.
